Sorting/SplaySort.v
@@ -27,32 +27,33 @@ Proof.
     rewrite e0 in IHp. cbn in IHp. rewrite IHp; trivial.
 Qed.*)
 
-Fixpoint fromList {A : LinDec} (l : list A) : SplayHeap A :=
+Fixpoint fromList {A : Type} (p : A -> A -> bool) (l : list A) : SplayHeap A :=
 match l with
     | [] => empty
-    | h :: t => insert h (fromList t)
+    | h :: t => insert p h (fromList p t)
 end.
 
-Definition splaySort (A : LinDec) (l : list A) : list A :=
-  BTree_toList (fromList l).
+Definition splaySort {A : Type} (p : A -> A -> bool) (l : list A) : list A :=
+  BTree_toList (fromList p l).
 
-(* TODO: fix isBST
+(*
 Lemma fromList_isBST :
-  forall (A : LinDec) (l : list A),
-    isBST (fromList l).
+  forall (A : LinDec) (p : A -> A -> comparison) (l : list A),
+    isBST p (fromList p l).
 Proof.
   induction l as [| h t]; cbn.
     constructor.
-    apply insert_isBST. assumption.
+    apply isBST_insert. assumption.
 Qed.
+*)
 
+(*
 Theorem Sorted_splaySort :
-  forall (A : LinDec) (l : list A),
-    Sorted A (splaySort A l).
+  forall (A : LinDec) (p : A -> A -> bool) (l : list A),
+    Sorted A (splaySort p l).
 Proof.
   intros. unfold splaySort. apply Sorted_BTree_toList, fromList_isBST.
 Qed.
-
 
 Lemma count_BTree_fromList :
   forall (A : LinDec) (p : A -> bool) (l : list A),
@@ -74,43 +75,43 @@ Qed.
 *)
 
 Lemma Permutation_partition :
-  forall (A : LinDec) (pivot : A) (h h1 h2 : SplayHeap A),
-    partition pivot h = (h1, h2) ->
+  forall (A : LinDec) (p : A -> A -> bool) (pivot : A) (h h1 h2 : SplayHeap A),
+    partition p pivot h = (h1, h2) ->
       Permutation (BTree_toList h) (BTree_toList h1 ++ BTree_toList h2).
 Proof.
-  intros A pivot h.
-  functional induction @partition A pivot h; cbn in *; intros.
+  intros A p pivot h.
+  functional induction @partition A p pivot h; cbn in *; intros.
     inv H.
     inv H. cbn. rewrite app_nil_r. reflexivity.
     inv H. cbn. rewrite <- !app_assoc. cbn. apply Permutation_app.
       reflexivity.
       constructor. apply Permutation_app.
         reflexivity.
-        constructor. apply IHp. assumption.
+        constructor. apply IHp0. assumption.
     inv H. cbn. rewrite <- !app_assoc. cbn. apply Permutation_app.
       reflexivity.
-      constructor. rewrite (IHp _ _ e3). rewrite <- !app_assoc. reflexivity.
+      constructor. rewrite (IHp0 _ _ e3). rewrite <- !app_assoc. reflexivity.
     inv H.
-    inv H. cbn. rewrite (IHp _ _ e3). rewrite <- !app_assoc. cbn.
+    inv H. cbn. rewrite (IHp0 _ _ e3). rewrite <- !app_assoc. cbn.
       rewrite <- app_assoc. reflexivity.
-    inv H. rewrite (IHp _ _ e3). cbn. rewrite <- !app_assoc. reflexivity.
+    inv H. rewrite (IHp0 _ _ e3). cbn. rewrite <- !app_assoc. reflexivity.
 Qed.
 
 Lemma Permutation_BTree_toList_insert :
-  forall (A : LinDec) (x : A) (t : BTree A),
-    Permutation (BTree_toList (insert x t)) (x :: BTree_toList t).
+  forall (A : LinDec) (p : A -> A -> bool) (x : A) (t : BTree A),
+    Permutation (BTree_toList (insert p x t)) (x :: BTree_toList t).
 Proof.
   induction t as [| v l r]; cbn.
     reflexivity.
-    unfold insert. destruct (partition x (node v l t1)) eqn: Heq.
+    unfold insert. destruct (partition p x (node v l t1)) eqn: Heq.
       cbn. rewrite Permutation_app_comm. cbn. constructor.
-        rewrite (@Permutation_partition _ _ _ _ _ Heq).
+        rewrite (@Permutation_partition _ _ _ _ _ _ Heq).
           apply Permutation_app_comm.
 Qed.
 
 Lemma Permutation_splaySort :
-  forall (A : LinDec) (l : list A),
-    Permutation (splaySort A l) l.
+  forall (A : LinDec) (p : A -> A -> bool) (l : list A),
+    Permutation (splaySort p l) l.
 Proof.
   intros. unfold splaySort.
   induction l as [| h t]; cbn.
